verif/trie/verif/verif_key.v
@@ -17,21 +17,13 @@ Import Coq.Lists.List.ListNotations.
 Definition Gprog : funspecs :=
   ltac:(with_library prog [
         surely_malloc_spec; (* KV_NewKey_spec; *)
-        KV_MoveKey_spec; KV_GetCharArray_spec;
-        KV_GetCharArraySize_spec
+        move_key_spec
        ]).
 
-Lemma body_KV_MoveKey: semax_body Vprog Gprog f_KV_MoveKey KV_MoveKey_spec.
+Lemma body_KV_MoveKey: semax_body Vprog Gprog f_move_key move_key_spec.
 Proof.
   start_function.
   forward.
-  forward_if (True);
-    [
-      unfold cstring_len;
-      forward_if (True);
-      [forward; entailer! | assert_PROP (False) by entailer!; contradiction] |
-      forward; entailer! |
-    ].
   forward_call (tkey).
   split3; auto; simpl; rep_omega.
   Intros k.
@@ -40,30 +32,6 @@ Proof.
   forward.
   Exists k.
   Exists s.
-  fold_keyrep.
-  entailer!.
-Qed.
-
-Lemma body_KV_GetCharArray: semax_body Vprog Gprog f_KV_GetCharArray KV_GetCharArray_spec.
-Proof.
-  start_function.
-  unfold key_rep.
-  Intros.
-  forward_if (True); [forward; entailer! | assert_PROP (False) by entailer!; contradiction | ].
-  forward.
-  forward.
-  fold_keyrep.
-  entailer!.
-Qed.
-
-Lemma body_KV_GetCharArraySize: semax_body Vprog Gprog f_KV_GetCharArraySize KV_GetCharArraySize_spec.
-Proof.
-  start_function.
-  unfold key_rep.
-  Intros.
-  forward_if (True); [forward; entailer! | assert_PROP (False) by entailer!; contradiction | ].
-  forward.
-  forward.
   fold_keyrep.
   entailer!.
 Qed.
