verif/trie/clight/index_string.v
@@ -1,0 +1,1839 @@
+From Coq Require Import String List ZArith.
+From compcert Require Import Coqlib Integers Floats AST Ctypes Cop Clight Clightdefs.
+Local Open Scope Z_scope.
+
+Definition _BN_CompareSuffix : ident := 113%positive.
+Definition _BN_ExportSuffixValue : ident := 108%positive.
+Definition _BN_FreeBorderNode : ident := 96%positive.
+Definition _BN_GetLink : ident := 110%positive.
+Definition _BN_GetPrefixValue : ident := 100%positive.
+Definition _BN_GetSuffixValue : ident := 106%positive.
+Definition _BN_HasSuffix : ident := 111%positive.
+Definition _BN_NewBorderNode : ident := 95%positive.
+Definition _BN_SetLink : ident := 109%positive.
+Definition _BN_SetPrefixValue : ident := 99%positive.
+Definition _BN_SetSuffixValue : ident := 102%positive.
+Definition _BN_SetValue : ident := 112%positive.
+Definition _BN_TestSuffix : ident := 104%positive.
+Definition _BorderNode : ident := 14%positive.
+Definition _CursorSlice_T : ident := 6%positive.
+Definition _Cursor_T : ident := 9%positive.
+Definition _Iget_key : ident := 71%positive.
+Definition _Iget_value : ident := 72%positive.
+Definition _Imake_cursor : ident := 70%positive.
+Definition _Key_T : ident := 3%positive.
+Definition _Sempty : ident := 115%positive.
+Definition _Smake_cursor : ident := 126%positive.
+Definition _UTIL_GetNextKeySlice : ident := 84%positive.
+Definition _UTIL_StrEqual : ident := 89%positive.
+Definition ___builtin_ais_annot : ident := 15%positive.
+Definition ___builtin_annot : ident := 22%positive.
+Definition ___builtin_annot_intval : ident := 23%positive.
+Definition ___builtin_bswap : ident := 16%positive.
+Definition ___builtin_bswap16 : ident := 18%positive.
+Definition ___builtin_bswap32 : ident := 17%positive.
+Definition ___builtin_bswap64 : ident := 48%positive.
+Definition ___builtin_clz : ident := 49%positive.
+Definition ___builtin_clzl : ident := 50%positive.
+Definition ___builtin_clzll : ident := 51%positive.
+Definition ___builtin_ctz : ident := 52%positive.
+Definition ___builtin_ctzl : ident := 53%positive.
+Definition ___builtin_ctzll : ident := 54%positive.
+Definition ___builtin_debug : ident := 66%positive.
+Definition ___builtin_fabs : ident := 19%positive.
+Definition ___builtin_fmadd : ident := 57%positive.
+Definition ___builtin_fmax : ident := 55%positive.
+Definition ___builtin_fmin : ident := 56%positive.
+Definition ___builtin_fmsub : ident := 58%positive.
+Definition ___builtin_fnmadd : ident := 59%positive.
+Definition ___builtin_fnmsub : ident := 60%positive.
+Definition ___builtin_fsqrt : ident := 20%positive.
+Definition ___builtin_membar : ident := 24%positive.
+Definition ___builtin_memcpy_aligned : ident := 21%positive.
+Definition ___builtin_nop : ident := 65%positive.
+Definition ___builtin_read16_reversed : ident := 61%positive.
+Definition ___builtin_read32_reversed : ident := 62%positive.
+Definition ___builtin_va_arg : ident := 26%positive.
+Definition ___builtin_va_copy : ident := 27%positive.
+Definition ___builtin_va_end : ident := 28%positive.
+Definition ___builtin_va_start : ident := 25%positive.
+Definition ___builtin_write16_reversed : ident := 63%positive.
+Definition ___builtin_write32_reversed : ident := 64%positive.
+Definition ___compcert_i64_dtos : ident := 33%positive.
+Definition ___compcert_i64_dtou : ident := 34%positive.
+Definition ___compcert_i64_sar : ident := 45%positive.
+Definition ___compcert_i64_sdiv : ident := 39%positive.
+Definition ___compcert_i64_shl : ident := 43%positive.
+Definition ___compcert_i64_shr : ident := 44%positive.
+Definition ___compcert_i64_smod : ident := 41%positive.
+Definition ___compcert_i64_smulh : ident := 46%positive.
+Definition ___compcert_i64_stod : ident := 35%positive.
+Definition ___compcert_i64_stof : ident := 37%positive.
+Definition ___compcert_i64_udiv : ident := 40%positive.
+Definition ___compcert_i64_umod : ident := 42%positive.
+Definition ___compcert_i64_umulh : ident := 47%positive.
+Definition ___compcert_i64_utod : ident := 36%positive.
+Definition ___compcert_i64_utof : ident := 38%positive.
+Definition ___compcert_va_composite : ident := 32%positive.
+Definition ___compcert_va_float64 : ident := 31%positive.
+Definition ___compcert_va_int32 : ident := 29%positive.
+Definition ___compcert_va_int64 : ident := 30%positive.
+Definition __make_cursor : ident := 125%positive.
+Definition _a : ident := 85%positive.
+Definition _b : ident := 87%positive.
+Definition _bn : ident := 97%positive.
+Definition _bnode : ident := 119%positive.
+Definition _bnode_cursor : ident := 5%positive.
+Definition _bordernode : ident := 94%positive.
+Definition _capacity : ident := 7%positive.
+Definition _content : ident := 1%positive.
+Definition _cursor : ident := 76%positive.
+Definition _exit : ident := 69%positive.
+Definition _free : ident := 68%positive.
+Definition _i : ident := 78%positive.
+Definition _index : ident := 116%positive.
+Definition _key : ident := 103%positive.
+Definition _keySuffix : ident := 12%positive.
+Definition _keySuffixLength : ident := 13%positive.
+Definition _keyslice : ident := 117%positive.
+Definition _len : ident := 2%positive.
+Definition _lenA : ident := 86%positive.
+Definition _lenB : ident := 88%positive.
+Definition _main : ident := 127%positive.
+Definition _malloc : ident := 67%positive.
+Definition _move_key : ident := 93%positive.
+Definition _n : ident := 73%positive.
+Definition _newKey : ident := 90%positive.
+Definition _newStr : ident := 91%positive.
+Definition _new_addr : ident := 77%positive.
+Definition _new_cursor : ident := 81%positive.
+Definition _new_index : ident := 114%positive.
+Definition _new_key : ident := 92%positive.
+Definition _node_cursor : ident := 4%positive.
+Definition _obtained_keyslice : ident := 118%positive.
+Definition _p : ident := 74%positive.
+Definition _pop_cursor : ident := 80%positive.
+Definition _prefixLinks : ident := 10%positive.
+Definition _push_cursor : ident := 79%positive.
+Definition _res : ident := 83%positive.
+Definition _ret_temp : ident := 107%positive.
+Definition _size : ident := 8%positive.
+Definition _slice : ident := 120%positive.
+Definition _slice__1 : ident := 123%positive.
+Definition _str : ident := 82%positive.
+Definition _subindex : ident := 122%positive.
+Definition _subkey : ident := 121%positive.
+Definition _subkey__1 : ident := 124%positive.
+Definition _suf : ident := 105%positive.
+Definition _suffix : ident := 101%positive.
+Definition _suffixLink : ident := 11%positive.
+Definition _surely_malloc : ident := 75%positive.
+Definition _val : ident := 98%positive.
+Definition _t'1 : ident := 128%positive.
+Definition _t'10 : ident := 137%positive.
+Definition _t'11 : ident := 138%positive.
+Definition _t'12 : ident := 139%positive.
+Definition _t'13 : ident := 140%positive.
+Definition _t'14 : ident := 141%positive.
+Definition _t'15 : ident := 142%positive.
+Definition _t'16 : ident := 143%positive.
+Definition _t'17 : ident := 144%positive.
+Definition _t'18 : ident := 145%positive.
+Definition _t'2 : ident := 129%positive.
+Definition _t'3 : ident := 130%positive.
+Definition _t'4 : ident := 131%positive.
+Definition _t'5 : ident := 132%positive.
+Definition _t'6 : ident := 133%positive.
+Definition _t'7 : ident := 134%positive.
+Definition _t'8 : ident := 135%positive.
+Definition _t'9 : ident := 136%positive.
+
+Definition f_surely_malloc := {|
+  fn_return := (tptr tvoid);
+  fn_callconv := cc_default;
+  fn_params := ((_n, tuint) :: nil);
+  fn_vars := nil;
+  fn_temps := ((_p, (tptr tvoid)) :: (_t'1, (tptr tvoid)) :: nil);
+  fn_body :=
+(Ssequence
+  (Ssequence
+    (Scall (Some _t'1)
+      (Evar _malloc (Tfunction (Tcons tuint Tnil) (tptr tvoid) cc_default))
+      ((Etempvar _n tuint) :: nil))
+    (Sset _p (Etempvar _t'1 (tptr tvoid))))
+  (Ssequence
+    (Sifthenelse (Eunop Onotbool (Etempvar _p (tptr tvoid)) tint)
+      (Scall None (Evar _exit (Tfunction (Tcons tint Tnil) tvoid cc_default))
+        ((Econst_int (Int.repr 1) tint) :: nil))
+      Sskip)
+    (Sreturn (Some (Etempvar _p (tptr tvoid))))))
+|}.
+
+Definition f_push_cursor := {|
+  fn_return := tvoid;
+  fn_callconv := cc_default;
+  fn_params := ((_node_cursor, (tptr tvoid)) :: (_bnode_cursor, tuint) ::
+                (_cursor, (tptr (Tstruct _Cursor_T noattr))) :: nil);
+  fn_vars := nil;
+  fn_temps := ((_new_addr, (tptr (Tstruct _CursorSlice_T noattr))) ::
+               (_i, tuint) :: (_t'2, (tptr tvoid)) :: (_t'1, (tptr tvoid)) ::
+               (_t'18, tuint) :: (_t'17, tuint) :: (_t'16, tuint) ::
+               (_t'15, (tptr tvoid)) ::
+               (_t'14, (tptr (Tstruct _CursorSlice_T noattr))) ::
+               (_t'13, tuint) ::
+               (_t'12, (tptr (Tstruct _CursorSlice_T noattr))) ::
+               (_t'11, (tptr (Tstruct _CursorSlice_T noattr))) ::
+               (_t'10, tuint) :: (_t'9, tuint) :: (_t'8, tuint) ::
+               (_t'7, tuint) ::
+               (_t'6, (tptr (Tstruct _CursorSlice_T noattr))) ::
+               (_t'5, tuint) ::
+               (_t'4, (tptr (Tstruct _CursorSlice_T noattr))) ::
+               (_t'3, tuint) :: nil);
+  fn_body :=
+(Ssequence
+  (Ssequence
+    (Sset _t'8
+      (Efield
+        (Ederef (Etempvar _cursor (tptr (Tstruct _Cursor_T noattr)))
+          (Tstruct _Cursor_T noattr)) _capacity tuint))
+    (Sifthenelse (Ebinop Oeq (Etempvar _t'8 tuint)
+                   (Econst_int (Int.repr 0) tint) tint)
+      (Ssequence
+        (Scall (Some _t'1)
+          (Evar _surely_malloc (Tfunction (Tcons tuint Tnil) (tptr tvoid)
+                                 cc_default))
+          ((Esizeof (Tstruct _CursorSlice_T noattr) tuint) :: nil))
+        (Sassign
+          (Efield
+            (Ederef (Etempvar _cursor (tptr (Tstruct _Cursor_T noattr)))
+              (Tstruct _Cursor_T noattr)) _content
+            (tptr (Tstruct _CursorSlice_T noattr)))
+          (Etempvar _t'1 (tptr tvoid))))
+      (Ssequence
+        (Sset _t'9
+          (Efield
+            (Ederef (Etempvar _cursor (tptr (Tstruct _Cursor_T noattr)))
+              (Tstruct _Cursor_T noattr)) _capacity tuint))
+        (Ssequence
+          (Sset _t'10
+            (Efield
+              (Ederef (Etempvar _cursor (tptr (Tstruct _Cursor_T noattr)))
+                (Tstruct _Cursor_T noattr)) _size tuint))
+          (Sifthenelse (Ebinop Ole (Etempvar _t'9 tuint)
+                         (Etempvar _t'10 tuint) tint)
+            (Ssequence
+              (Ssequence
+                (Sset _t'18
+                  (Efield
+                    (Ederef
+                      (Etempvar _cursor (tptr (Tstruct _Cursor_T noattr)))
+                      (Tstruct _Cursor_T noattr)) _capacity tuint))
+                (Sassign
+                  (Efield
+                    (Ederef
+                      (Etempvar _cursor (tptr (Tstruct _Cursor_T noattr)))
+                      (Tstruct _Cursor_T noattr)) _capacity tuint)
+                  (Ebinop Omul (Etempvar _t'18 tuint)
+                    (Econst_int (Int.repr 2) tint) tuint)))
+              (Ssequence
+                (Ssequence
+                  (Ssequence
+                    (Sset _t'17
+                      (Efield
+                        (Ederef
+                          (Etempvar _cursor (tptr (Tstruct _Cursor_T noattr)))
+                          (Tstruct _Cursor_T noattr)) _capacity tuint))
+                    (Scall (Some _t'2)
+                      (Evar _surely_malloc (Tfunction (Tcons tuint Tnil)
+                                             (tptr tvoid) cc_default))
+                      ((Ebinop Omul
+                         (Esizeof (Tstruct _CursorSlice_T noattr) tuint)
+                         (Etempvar _t'17 tuint) tuint) :: nil)))
+                  (Sset _new_addr (Etempvar _t'2 (tptr tvoid))))
+                (Ssequence
+                  (Ssequence
+                    (Sset _i (Econst_int (Int.repr 0) tint))
+                    (Sloop
+                      (Ssequence
+                        (Ssequence
+                          (Sset _t'16
+                            (Efield
+                              (Ederef
+                                (Etempvar _cursor (tptr (Tstruct _Cursor_T noattr)))
+                                (Tstruct _Cursor_T noattr)) _size tuint))
+                          (Sifthenelse (Ebinop Olt (Etempvar _i tuint)
+                                         (Etempvar _t'16 tuint) tint)
+                            Sskip
+                            Sbreak))
+                        (Ssequence
+                          (Ssequence
+                            (Sset _t'14
+                              (Efield
+                                (Ederef
+                                  (Etempvar _cursor (tptr (Tstruct _Cursor_T noattr)))
+                                  (Tstruct _Cursor_T noattr)) _content
+                                (tptr (Tstruct _CursorSlice_T noattr))))
+                            (Ssequence
+                              (Sset _t'15
+                                (Efield
+                                  (Ederef
+                                    (Ebinop Oadd
+                                      (Etempvar _t'14 (tptr (Tstruct _CursorSlice_T noattr)))
+                                      (Etempvar _i tuint)
+                                      (tptr (Tstruct _CursorSlice_T noattr)))
+                                    (Tstruct _CursorSlice_T noattr))
+                                  _node_cursor (tptr tvoid)))
+                              (Sassign
+                                (Efield
+                                  (Ederef
+                                    (Ebinop Oadd
+                                      (Etempvar _new_addr (tptr (Tstruct _CursorSlice_T noattr)))
+                                      (Etempvar _i tuint)
+                                      (tptr (Tstruct _CursorSlice_T noattr)))
+                                    (Tstruct _CursorSlice_T noattr))
+                                  _node_cursor (tptr tvoid))
+                                (Etempvar _t'15 (tptr tvoid)))))
+                          (Ssequence
+                            (Sset _t'12
+                              (Efield
+                                (Ederef
+                                  (Etempvar _cursor (tptr (Tstruct _Cursor_T noattr)))
+                                  (Tstruct _Cursor_T noattr)) _content
+                                (tptr (Tstruct _CursorSlice_T noattr))))
+                            (Ssequence
+                              (Sset _t'13
+                                (Efield
+                                  (Ederef
+                                    (Ebinop Oadd
+                                      (Etempvar _t'12 (tptr (Tstruct _CursorSlice_T noattr)))
+                                      (Etempvar _i tuint)
+                                      (tptr (Tstruct _CursorSlice_T noattr)))
+                                    (Tstruct _CursorSlice_T noattr))
+                                  _bnode_cursor tuint))
+                              (Sassign
+                                (Efield
+                                  (Ederef
+                                    (Ebinop Oadd
+                                      (Etempvar _new_addr (tptr (Tstruct _CursorSlice_T noattr)))
+                                      (Etempvar _i tuint)
+                                      (tptr (Tstruct _CursorSlice_T noattr)))
+                                    (Tstruct _CursorSlice_T noattr))
+                                  _bnode_cursor tuint)
+                                (Etempvar _t'13 tuint))))))
+                      (Sset _i
+                        (Ebinop Oadd (Etempvar _i tuint)
+                          (Econst_int (Int.repr 1) tint) tuint))))
+                  (Ssequence
+                    (Ssequence
+                      (Sset _t'11
+                        (Efield
+                          (Ederef
+                            (Etempvar _cursor (tptr (Tstruct _Cursor_T noattr)))
+                            (Tstruct _Cursor_T noattr)) _content
+                          (tptr (Tstruct _CursorSlice_T noattr))))
+                      (Scall None
+                        (Evar _free (Tfunction (Tcons (tptr tvoid) Tnil)
+                                      tvoid cc_default))
+                        ((Etempvar _t'11 (tptr (Tstruct _CursorSlice_T noattr))) ::
+                         nil)))
+                    (Sassign
+                      (Efield
+                        (Ederef
+                          (Etempvar _cursor (tptr (Tstruct _Cursor_T noattr)))
+                          (Tstruct _Cursor_T noattr)) _content
+                        (tptr (Tstruct _CursorSlice_T noattr)))
+                      (Etempvar _new_addr (tptr (Tstruct _CursorSlice_T noattr))))))))
+            Sskip)))))
+  (Ssequence
+    (Ssequence
+      (Sset _t'6
+        (Efield
+          (Ederef (Etempvar _cursor (tptr (Tstruct _Cursor_T noattr)))
+            (Tstruct _Cursor_T noattr)) _content
+          (tptr (Tstruct _CursorSlice_T noattr))))
+      (Ssequence
+        (Sset _t'7
+          (Efield
+            (Ederef (Etempvar _cursor (tptr (Tstruct _Cursor_T noattr)))
+              (Tstruct _Cursor_T noattr)) _size tuint))
+        (Sassign
+          (Efield
+            (Ederef
+              (Ebinop Oadd
+                (Etempvar _t'6 (tptr (Tstruct _CursorSlice_T noattr)))
+                (Etempvar _t'7 tuint) (tptr (Tstruct _CursorSlice_T noattr)))
+              (Tstruct _CursorSlice_T noattr)) _node_cursor (tptr tvoid))
+          (Etempvar _node_cursor (tptr tvoid)))))
+    (Ssequence
+      (Ssequence
+        (Sset _t'4
+          (Efield
+            (Ederef (Etempvar _cursor (tptr (Tstruct _Cursor_T noattr)))
+              (Tstruct _Cursor_T noattr)) _content
+            (tptr (Tstruct _CursorSlice_T noattr))))
+        (Ssequence
+          (Sset _t'5
+            (Efield
+              (Ederef (Etempvar _cursor (tptr (Tstruct _Cursor_T noattr)))
+                (Tstruct _Cursor_T noattr)) _size tuint))
+          (Sassign
+            (Efield
+              (Ederef
+                (Ebinop Oadd
+                  (Etempvar _t'4 (tptr (Tstruct _CursorSlice_T noattr)))
+                  (Etempvar _t'5 tuint)
+                  (tptr (Tstruct _CursorSlice_T noattr)))
+                (Tstruct _CursorSlice_T noattr)) _bnode_cursor tuint)
+            (Etempvar _bnode_cursor tuint))))
+      (Ssequence
+        (Sset _t'3
+          (Efield
+            (Ederef (Etempvar _cursor (tptr (Tstruct _Cursor_T noattr)))
+              (Tstruct _Cursor_T noattr)) _size tuint))
+        (Sassign
+          (Efield
+            (Ederef (Etempvar _cursor (tptr (Tstruct _Cursor_T noattr)))
+              (Tstruct _Cursor_T noattr)) _size tuint)
+          (Ebinop Oadd (Etempvar _t'3 tuint) (Econst_int (Int.repr 1) tint)
+            tuint))))))
+|}.
+
+Definition f_pop_cursor := {|
+  fn_return := tvoid;
+  fn_callconv := cc_default;
+  fn_params := ((_cursor, (tptr (Tstruct _Cursor_T noattr))) :: nil);
+  fn_vars := nil;
+  fn_temps := ((_t'1, tuint) :: nil);
+  fn_body :=
+(Ssequence
+  (Sset _t'1
+    (Efield
+      (Ederef (Etempvar _cursor (tptr (Tstruct _Cursor_T noattr)))
+        (Tstruct _Cursor_T noattr)) _size tuint))
+  (Sassign
+    (Efield
+      (Ederef (Etempvar _cursor (tptr (Tstruct _Cursor_T noattr)))
+        (Tstruct _Cursor_T noattr)) _size tuint)
+    (Ebinop Osub (Etempvar _t'1 tuint) (Econst_int (Int.repr 1) tint) tuint)))
+|}.
+
+Definition f_new_cursor := {|
+  fn_return := (tptr (Tstruct _Cursor_T noattr));
+  fn_callconv := cc_default;
+  fn_params := nil;
+  fn_vars := nil;
+  fn_temps := ((_cursor, (tptr (Tstruct _Cursor_T noattr))) ::
+               (_t'2, tuint) :: (_t'1, (tptr tvoid)) :: nil);
+  fn_body :=
+(Ssequence
+  (Ssequence
+    (Scall (Some _t'1)
+      (Evar _surely_malloc (Tfunction (Tcons tuint Tnil) (tptr tvoid)
+                             cc_default))
+      ((Esizeof (tptr (Tstruct _Cursor_T noattr)) tuint) :: nil))
+    (Sset _cursor (Etempvar _t'1 (tptr tvoid))))
+  (Ssequence
+    (Ssequence
+      (Ssequence
+        (Sset _t'2 (Ecast (Econst_int (Int.repr 0) tint) tuint))
+        (Sassign
+          (Efield
+            (Ederef (Etempvar _cursor (tptr (Tstruct _Cursor_T noattr)))
+              (Tstruct _Cursor_T noattr)) _size tuint) (Etempvar _t'2 tuint)))
+      (Sassign
+        (Efield
+          (Ederef (Etempvar _cursor (tptr (Tstruct _Cursor_T noattr)))
+            (Tstruct _Cursor_T noattr)) _capacity tuint)
+        (Etempvar _t'2 tuint)))
+    (Ssequence
+      (Sassign
+        (Efield
+          (Ederef (Etempvar _cursor (tptr (Tstruct _Cursor_T noattr)))
+            (Tstruct _Cursor_T noattr)) _content
+          (tptr (Tstruct _CursorSlice_T noattr)))
+        (Econst_int (Int.repr 0) tint))
+      (Sreturn (Some (Etempvar _cursor (tptr (Tstruct _Cursor_T noattr))))))))
+|}.
+
+Definition f_UTIL_GetNextKeySlice := {|
+  fn_return := tuint;
+  fn_callconv := cc_default;
+  fn_params := ((_str, (tptr tschar)) :: (_len, tint) :: nil);
+  fn_vars := nil;
+  fn_temps := ((_res, tuint) :: (_i, tint) :: (_t'1, tschar) :: nil);
+  fn_body :=
+(Ssequence
+  (Sset _res (Econst_int (Int.repr 0) tint))
+  (Ssequence
+    (Sset _i (Econst_int (Int.repr 0) tint))
+    (Ssequence
+      (Swhile
+        (Ebinop Olt (Etempvar _i tint) (Etempvar _len tint) tint)
+        (Ssequence
+          (Sset _res
+            (Ebinop Oshl (Etempvar _res tuint) (Econst_int (Int.repr 8) tint)
+              tuint))
+          (Ssequence
+            (Ssequence
+              (Sset _t'1 (Ederef (Etempvar _str (tptr tschar)) tschar))
+              (Sset _res
+                (Ebinop Oor (Etempvar _res tuint)
+                  (Ebinop Oand (Ecast (Etempvar _t'1 tschar) tuint)
+                    (Econst_int (Int.repr 255) tint) tuint) tuint)))
+            (Ssequence
+              (Sset _str
+                (Ebinop Oadd (Etempvar _str (tptr tschar))
+                  (Econst_int (Int.repr 1) tint) (tptr tschar)))
+              (Sset _i
+                (Ebinop Oadd (Etempvar _i tint)
+                  (Econst_int (Int.repr 1) tint) tint))))))
+      (Ssequence
+        (Swhile
+          (Ebinop Olt (Etempvar _i tint) (Ecast (Esizeof tuint tuint) tint)
+            tint)
+          (Ssequence
+            (Sset _res
+              (Ebinop Oshl (Etempvar _res tuint)
+                (Econst_int (Int.repr 8) tint) tuint))
+            (Sset _i
+              (Ebinop Oadd (Etempvar _i tint) (Econst_int (Int.repr 1) tint)
+                tint))))
+        (Sreturn (Some (Etempvar _res tuint)))))))
+|}.
+
+Definition f_UTIL_StrEqual := {|
+  fn_return := tint;
+  fn_callconv := cc_default;
+  fn_params := ((_a, (tptr tschar)) :: (_lenA, tuint) ::
+                (_b, (tptr tschar)) :: (_lenB, tuint) :: nil);
+  fn_vars := nil;
+  fn_temps := ((_i, tuint) :: (_t'2, tschar) :: (_t'1, tschar) :: nil);
+  fn_body :=
+(Ssequence
+  (Sifthenelse (Ebinop One (Etempvar _lenA tuint) (Etempvar _lenB tuint)
+                 tint)
+    (Sreturn (Some (Econst_int (Int.repr 0) tint)))
+    Sskip)
+  (Ssequence
+    (Ssequence
+      (Sset _i (Econst_int (Int.repr 0) tint))
+      (Sloop
+        (Ssequence
+          (Sifthenelse (Ebinop Olt (Etempvar _i tuint) (Etempvar _lenA tuint)
+                         tint)
+            Sskip
+            Sbreak)
+          (Ssequence
+            (Sset _t'1
+              (Ederef
+                (Ebinop Oadd (Etempvar _a (tptr tschar)) (Etempvar _i tuint)
+                  (tptr tschar)) tschar))
+            (Ssequence
+              (Sset _t'2
+                (Ederef
+                  (Ebinop Oadd (Etempvar _b (tptr tschar))
+                    (Etempvar _i tuint) (tptr tschar)) tschar))
+              (Sifthenelse (Ebinop One (Etempvar _t'1 tschar)
+                             (Etempvar _t'2 tschar) tint)
+                (Sreturn (Some (Econst_int (Int.repr 0) tint)))
+                Sskip))))
+        (Sset _i
+          (Ebinop Oadd (Etempvar _i tuint) (Econst_int (Int.repr 1) tint)
+            tuint))))
+    (Sreturn (Some (Econst_int (Int.repr 1) tint)))))
+|}.
+
+Definition f_new_key := {|
+  fn_return := (tptr (Tstruct _Key_T noattr));
+  fn_callconv := cc_default;
+  fn_params := ((_str, (tptr tschar)) :: (_len, tuint) :: nil);
+  fn_vars := nil;
+  fn_temps := ((_newKey, (tptr (Tstruct _Key_T noattr))) ::
+               (_newStr, (tptr tschar)) :: (_i, tuint) ::
+               (_t'2, (tptr tvoid)) :: (_t'1, (tptr tvoid)) ::
+               (_t'3, tschar) :: nil);
+  fn_body :=
+(Ssequence
+  (Sset _newKey
+    (Ecast (Econst_int (Int.repr 0) tint) (tptr (Tstruct _Key_T noattr))))
+  (Ssequence
+    (Ssequence
+      (Scall (Some _t'1)
+        (Evar _surely_malloc (Tfunction (Tcons tuint Tnil) (tptr tvoid)
+                               cc_default))
+        ((Ebinop Omul (Esizeof tschar tuint) (Etempvar _len tuint) tuint) ::
+         nil))
+      (Sset _newStr (Ecast (Etempvar _t'1 (tptr tvoid)) (tptr tschar))))
+    (Ssequence
+      (Ssequence
+        (Sset _i (Econst_int (Int.repr 0) tint))
+        (Sloop
+          (Ssequence
+            (Sifthenelse (Ebinop Olt (Etempvar _i tuint)
+                           (Etempvar _len tuint) tint)
+              Sskip
+              Sbreak)
+            (Ssequence
+              (Sset _t'3
+                (Ederef
+                  (Ebinop Oadd (Etempvar _str (tptr tschar))
+                    (Etempvar _i tuint) (tptr tschar)) tschar))
+              (Sassign
+                (Ederef
+                  (Ebinop Oadd (Etempvar _newStr (tptr tschar))
+                    (Etempvar _i tuint) (tptr tschar)) tschar)
+                (Etempvar _t'3 tschar))))
+          (Sset _i
+            (Ebinop Oadd (Etempvar _i tuint) (Econst_int (Int.repr 1) tint)
+              tuint))))
+      (Ssequence
+        (Ssequence
+          (Scall (Some _t'2)
+            (Evar _surely_malloc (Tfunction (Tcons tuint Tnil) (tptr tvoid)
+                                   cc_default))
+            ((Esizeof (Tstruct _Key_T noattr) tuint) :: nil))
+          (Sset _newKey
+            (Ecast (Etempvar _t'2 (tptr tvoid))
+              (tptr (Tstruct _Key_T noattr)))))
+        (Ssequence
+          (Sassign
+            (Efield
+              (Ederef (Etempvar _newKey (tptr (Tstruct _Key_T noattr)))
+                (Tstruct _Key_T noattr)) _content (tptr tschar))
+            (Etempvar _newStr (tptr tschar)))
+          (Ssequence
+            (Sassign
+              (Efield
+                (Ederef (Etempvar _newKey (tptr (Tstruct _Key_T noattr)))
+                  (Tstruct _Key_T noattr)) _len tuint) (Etempvar _len tuint))
+            (Sreturn (Some (Etempvar _newKey (tptr (Tstruct _Key_T noattr)))))))))))
+|}.
+
+Definition f_move_key := {|
+  fn_return := (tptr (Tstruct _Key_T noattr));
+  fn_callconv := cc_default;
+  fn_params := ((_str, (tptr tschar)) :: (_len, tuint) :: nil);
+  fn_vars := nil;
+  fn_temps := ((_newKey, (tptr (Tstruct _Key_T noattr))) ::
+               (_t'1, (tptr tvoid)) :: nil);
+  fn_body :=
+(Ssequence
+  (Sset _newKey
+    (Ecast (Econst_int (Int.repr 0) tint) (tptr (Tstruct _Key_T noattr))))
+  (Ssequence
+    (Ssequence
+      (Scall (Some _t'1)
+        (Evar _surely_malloc (Tfunction (Tcons tuint Tnil) (tptr tvoid)
+                               cc_default))
+        ((Esizeof (Tstruct _Key_T noattr) tuint) :: nil))
+      (Sset _newKey
+        (Ecast (Etempvar _t'1 (tptr tvoid)) (tptr (Tstruct _Key_T noattr)))))
+    (Ssequence
+      (Sassign
+        (Efield
+          (Ederef (Etempvar _newKey (tptr (Tstruct _Key_T noattr)))
+            (Tstruct _Key_T noattr)) _content (tptr tschar))
+        (Etempvar _str (tptr tschar)))
+      (Ssequence
+        (Sassign
+          (Efield
+            (Ederef (Etempvar _newKey (tptr (Tstruct _Key_T noattr)))
+              (Tstruct _Key_T noattr)) _len tuint) (Etempvar _len tuint))
+        (Sreturn (Some (Etempvar _newKey (tptr (Tstruct _Key_T noattr)))))))))
+|}.
+
+Definition f_BN_NewBorderNode := {|
+  fn_return := (tptr (Tstruct _BorderNode noattr));
+  fn_callconv := cc_default;
+  fn_params := nil;
+  fn_vars := nil;
+  fn_temps := ((_bordernode, (tptr (Tstruct _BorderNode noattr))) ::
+               (_i, tint) :: (_t'1, (tptr tvoid)) :: nil);
+  fn_body :=
+(Ssequence
+  (Ssequence
+    (Scall (Some _t'1)
+      (Evar _surely_malloc (Tfunction (Tcons tuint Tnil) (tptr tvoid)
+                             cc_default))
+      ((Esizeof (Tstruct _BorderNode noattr) tuint) :: nil))
+    (Sset _bordernode
+      (Ecast (Etempvar _t'1 (tptr tvoid))
+        (tptr (Tstruct _BorderNode noattr)))))
+  (Ssequence
+    (Ssequence
+      (Sset _i (Econst_int (Int.repr 0) tint))
+      (Sloop
+        (Ssequence
+          (Sifthenelse (Ebinop Olt (Etempvar _i tint)
+                         (Econst_int (Int.repr 4) tint) tint)
+            Sskip
+            Sbreak)
+          (Sassign
+            (Ederef
+              (Ebinop Oadd
+                (Efield
+                  (Ederef
+                    (Etempvar _bordernode (tptr (Tstruct _BorderNode noattr)))
+                    (Tstruct _BorderNode noattr)) _prefixLinks
+                  (tarray (tptr tvoid) 4)) (Etempvar _i tint)
+                (tptr (tptr tvoid))) (tptr tvoid))
+            (Econst_int (Int.repr 0) tint)))
+        (Sset _i
+          (Ebinop Oadd (Etempvar _i tint) (Econst_int (Int.repr 1) tint)
+            tint))))
+    (Ssequence
+      (Sassign
+        (Efield
+          (Ederef (Etempvar _bordernode (tptr (Tstruct _BorderNode noattr)))
+            (Tstruct _BorderNode noattr)) _suffixLink (tptr tvoid))
+        (Econst_int (Int.repr 0) tint))
+      (Ssequence
+        (Sassign
+          (Efield
+            (Ederef
+              (Etempvar _bordernode (tptr (Tstruct _BorderNode noattr)))
+              (Tstruct _BorderNode noattr)) _keySuffix (tptr tschar))
+          (Econst_int (Int.repr 0) tint))
+        (Ssequence
+          (Sassign
+            (Efield
+              (Ederef
+                (Etempvar _bordernode (tptr (Tstruct _BorderNode noattr)))
+                (Tstruct _BorderNode noattr)) _keySuffixLength tuint)
+            (Econst_int (Int.repr 0) tint))
+          (Sreturn (Some (Etempvar _bordernode (tptr (Tstruct _BorderNode noattr))))))))))
+|}.
+
+Definition f_BN_FreeBorderNode := {|
+  fn_return := tvoid;
+  fn_callconv := cc_default;
+  fn_params := ((_bordernode, (tptr (Tstruct _BorderNode noattr))) :: nil);
+  fn_vars := nil;
+  fn_temps := ((_t'2, (tptr tschar)) :: (_t'1, (tptr tschar)) :: nil);
+  fn_body :=
+(Ssequence
+  (Sifthenelse (Ebinop Oeq
+                 (Etempvar _bordernode (tptr (Tstruct _BorderNode noattr)))
+                 (Ecast (Econst_int (Int.repr 0) tint) (tptr tvoid)) tint)
+    (Sreturn None)
+    Sskip)
+  (Ssequence
+    (Ssequence
+      (Sset _t'1
+        (Efield
+          (Ederef (Etempvar _bordernode (tptr (Tstruct _BorderNode noattr)))
+            (Tstruct _BorderNode noattr)) _keySuffix (tptr tschar)))
+      (Sifthenelse (Ebinop One (Etempvar _t'1 (tptr tschar))
+                     (Ecast (Econst_int (Int.repr 0) tint) (tptr tvoid))
+                     tint)
+        (Ssequence
+          (Sset _t'2
+            (Efield
+              (Ederef
+                (Etempvar _bordernode (tptr (Tstruct _BorderNode noattr)))
+                (Tstruct _BorderNode noattr)) _keySuffix (tptr tschar)))
+          (Scall None
+            (Evar _free (Tfunction (Tcons (tptr tvoid) Tnil) tvoid
+                          cc_default))
+            ((Etempvar _t'2 (tptr tschar)) :: nil)))
+        Sskip))
+    (Ssequence
+      (Scall None
+        (Evar _free (Tfunction (Tcons (tptr tvoid) Tnil) tvoid cc_default))
+        ((Etempvar _bordernode (tptr (Tstruct _BorderNode noattr))) :: nil))
+      (Sreturn None))))
+|}.
+
+Definition f_BN_SetPrefixValue := {|
+  fn_return := tvoid;
+  fn_callconv := cc_default;
+  fn_params := ((_bn, (tptr (Tstruct _BorderNode noattr))) :: (_i, tint) ::
+                (_val, (tptr tvoid)) :: nil);
+  fn_vars := nil;
+  fn_temps := nil;
+  fn_body :=
+(Sassign
+  (Ederef
+    (Ebinop Oadd
+      (Efield
+        (Ederef (Etempvar _bn (tptr (Tstruct _BorderNode noattr)))
+          (Tstruct _BorderNode noattr)) _prefixLinks (tarray (tptr tvoid) 4))
+      (Ebinop Osub (Etempvar _i tint) (Econst_int (Int.repr 1) tint) tint)
+      (tptr (tptr tvoid))) (tptr tvoid)) (Etempvar _val (tptr tvoid)))
+|}.
+
+Definition f_BN_GetPrefixValue := {|
+  fn_return := (tptr tvoid);
+  fn_callconv := cc_default;
+  fn_params := ((_bn, (tptr (Tstruct _BorderNode noattr))) :: (_i, tint) ::
+                nil);
+  fn_vars := nil;
+  fn_temps := ((_t'1, (tptr tvoid)) :: nil);
+  fn_body :=
+(Ssequence
+  (Sset _t'1
+    (Ederef
+      (Ebinop Oadd
+        (Efield
+          (Ederef (Etempvar _bn (tptr (Tstruct _BorderNode noattr)))
+            (Tstruct _BorderNode noattr)) _prefixLinks
+          (tarray (tptr tvoid) 4))
+        (Ebinop Osub (Etempvar _i tint) (Econst_int (Int.repr 1) tint) tint)
+        (tptr (tptr tvoid))) (tptr tvoid)))
+  (Sreturn (Some (Etempvar _t'1 (tptr tvoid)))))
+|}.
+
+Definition f_BN_SetSuffixValue := {|
+  fn_return := tvoid;
+  fn_callconv := cc_default;
+  fn_params := ((_bn, (tptr (Tstruct _BorderNode noattr))) ::
+                (_suffix, (tptr tschar)) :: (_len, tuint) ::
+                (_val, (tptr tvoid)) :: nil);
+  fn_vars := nil;
+  fn_temps := ((_i, tuint) :: (_t'1, (tptr tvoid)) ::
+               (_t'5, (tptr tschar)) :: (_t'4, (tptr tschar)) ::
+               (_t'3, tschar) :: (_t'2, (tptr tschar)) :: nil);
+  fn_body :=
+(Ssequence
+  (Ssequence
+    (Sset _t'4
+      (Efield
+        (Ederef (Etempvar _bn (tptr (Tstruct _BorderNode noattr)))
+          (Tstruct _BorderNode noattr)) _keySuffix (tptr tschar)))
+    (Sifthenelse (Ebinop One (Etempvar _t'4 (tptr tschar))
+                   (Ecast (Econst_int (Int.repr 0) tint) (tptr tvoid)) tint)
+      (Ssequence
+        (Sset _t'5
+          (Efield
+            (Ederef (Etempvar _bn (tptr (Tstruct _BorderNode noattr)))
+              (Tstruct _BorderNode noattr)) _keySuffix (tptr tschar)))
+        (Scall None
+          (Evar _free (Tfunction (Tcons (tptr tvoid) Tnil) tvoid cc_default))
+          ((Etempvar _t'5 (tptr tschar)) :: nil)))
+      Sskip))
+  (Ssequence
+    (Ssequence
+      (Scall (Some _t'1)
+        (Evar _surely_malloc (Tfunction (Tcons tuint Tnil) (tptr tvoid)
+                               cc_default))
+        ((Ebinop Omul (Esizeof tschar tuint) (Etempvar _len tuint) tuint) ::
+         nil))
+      (Sassign
+        (Efield
+          (Ederef (Etempvar _bn (tptr (Tstruct _BorderNode noattr)))
+            (Tstruct _BorderNode noattr)) _keySuffix (tptr tschar))
+        (Ecast (Etempvar _t'1 (tptr tvoid)) (tptr tschar))))
+    (Ssequence
+      (Ssequence
+        (Sset _i (Econst_int (Int.repr 0) tint))
+        (Sloop
+          (Ssequence
+            (Sifthenelse (Ebinop Olt (Etempvar _i tuint)
+                           (Etempvar _len tuint) tint)
+              Sskip
+              Sbreak)
+            (Ssequence
+              (Sset _t'2
+                (Efield
+                  (Ederef (Etempvar _bn (tptr (Tstruct _BorderNode noattr)))
+                    (Tstruct _BorderNode noattr)) _keySuffix (tptr tschar)))
+              (Ssequence
+                (Sset _t'3
+                  (Ederef
+                    (Ebinop Oadd (Etempvar _suffix (tptr tschar))
+                      (Etempvar _i tuint) (tptr tschar)) tschar))
+                (Sassign
+                  (Ederef
+                    (Ebinop Oadd (Etempvar _t'2 (tptr tschar))
+                      (Etempvar _i tuint) (tptr tschar)) tschar)
+                  (Etempvar _t'3 tschar)))))
+          (Sset _i
+            (Ebinop Oadd (Etempvar _i tuint) (Econst_int (Int.repr 1) tint)
+              tuint))))
+      (Ssequence
+        (Sassign
+          (Efield
+            (Ederef (Etempvar _bn (tptr (Tstruct _BorderNode noattr)))
+              (Tstruct _BorderNode noattr)) _keySuffixLength tuint)
+          (Etempvar _len tuint))
+        (Sassign
+          (Efield
+            (Ederef (Etempvar _bn (tptr (Tstruct _BorderNode noattr)))
+              (Tstruct _BorderNode noattr)) _suffixLink (tptr tvoid))
+          (Etempvar _val (tptr tvoid)))))))
+|}.
+
+Definition f_BN_TestSuffix := {|
+  fn_return := tint;
+  fn_callconv := cc_default;
+  fn_params := ((_bn, (tptr (Tstruct _BorderNode noattr))) ::
+                (_key, (tptr (Tstruct _Key_T noattr))) :: nil);
+  fn_vars := nil;
+  fn_temps := ((_t'1, tint) :: (_t'6, tuint) :: (_t'5, (tptr tschar)) ::
+               (_t'4, tuint) :: (_t'3, (tptr tschar)) ::
+               (_t'2, (tptr tschar)) :: nil);
+  fn_body :=
+(Ssequence
+  (Sset _t'2
+    (Efield
+      (Ederef (Etempvar _bn (tptr (Tstruct _BorderNode noattr)))
+        (Tstruct _BorderNode noattr)) _keySuffix (tptr tschar)))
+  (Sifthenelse (Ebinop One (Etempvar _t'2 (tptr tschar))
+                 (Ecast (Econst_int (Int.repr 0) tint) (tptr tvoid)) tint)
+    (Ssequence
+      (Ssequence
+        (Sset _t'3
+          (Efield
+            (Ederef (Etempvar _key (tptr (Tstruct _Key_T noattr)))
+              (Tstruct _Key_T noattr)) _content (tptr tschar)))
+        (Ssequence
+          (Sset _t'4
+            (Efield
+              (Ederef (Etempvar _key (tptr (Tstruct _Key_T noattr)))
+                (Tstruct _Key_T noattr)) _len tuint))
+          (Ssequence
+            (Sset _t'5
+              (Efield
+                (Ederef (Etempvar _bn (tptr (Tstruct _BorderNode noattr)))
+                  (Tstruct _BorderNode noattr)) _keySuffix (tptr tschar)))
+            (Ssequence
+              (Sset _t'6
+                (Efield
+                  (Ederef (Etempvar _bn (tptr (Tstruct _BorderNode noattr)))
+                    (Tstruct _BorderNode noattr)) _keySuffixLength tuint))
+              (Scall (Some _t'1)
+                (Evar _UTIL_StrEqual (Tfunction
+                                       (Tcons (tptr tschar)
+                                         (Tcons tuint
+                                           (Tcons (tptr tschar)
+                                             (Tcons tuint Tnil)))) tint
+                                       cc_default))
+                ((Ebinop Oadd (Etempvar _t'3 (tptr tschar))
+                   (Ecast (Esizeof tuint tuint) tint) (tptr tschar)) ::
+                 (Ebinop Osub (Etempvar _t'4 tuint)
+                   (Ecast (Esizeof tuint tuint) tint) tuint) ::
+                 (Etempvar _t'5 (tptr tschar)) :: (Etempvar _t'6 tuint) ::
+                 nil))))))
+      (Sreturn (Some (Etempvar _t'1 tint))))
+    (Sreturn (Some (Econst_int (Int.repr 0) tint)))))
+|}.
+
+Definition f_BN_GetSuffixValue := {|
+  fn_return := (tptr tvoid);
+  fn_callconv := cc_default;
+  fn_params := ((_bn, (tptr (Tstruct _BorderNode noattr))) ::
+                (_suf, (tptr tschar)) :: (_len, tuint) :: nil);
+  fn_vars := nil;
+  fn_temps := ((_t'1, tint) :: (_t'5, (tptr tschar)) :: (_t'4, tuint) ::
+               (_t'3, (tptr tschar)) :: (_t'2, (tptr tvoid)) :: nil);
+  fn_body :=
+(Ssequence
+  (Ssequence
+    (Sset _t'5
+      (Efield
+        (Ederef (Etempvar _bn (tptr (Tstruct _BorderNode noattr)))
+          (Tstruct _BorderNode noattr)) _keySuffix (tptr tschar)))
+    (Sifthenelse (Ebinop Oeq (Etempvar _t'5 (tptr tschar))
+                   (Ecast (Econst_int (Int.repr 0) tint) (tptr tvoid)) tint)
+      (Sreturn (Some (Econst_int (Int.repr 0) tint)))
+      Sskip))
+  (Ssequence
+    (Ssequence
+      (Sset _t'3
+        (Efield
+          (Ederef (Etempvar _bn (tptr (Tstruct _BorderNode noattr)))
+            (Tstruct _BorderNode noattr)) _keySuffix (tptr tschar)))
+      (Ssequence
+        (Sset _t'4
+          (Efield
+            (Ederef (Etempvar _bn (tptr (Tstruct _BorderNode noattr)))
+              (Tstruct _BorderNode noattr)) _keySuffixLength tuint))
+        (Scall (Some _t'1)
+          (Evar _UTIL_StrEqual (Tfunction
+                                 (Tcons (tptr tschar)
+                                   (Tcons tuint
+                                     (Tcons (tptr tschar) (Tcons tuint Tnil))))
+                                 tint cc_default))
+          ((Etempvar _suf (tptr tschar)) :: (Etempvar _len tuint) ::
+           (Etempvar _t'3 (tptr tschar)) :: (Etempvar _t'4 tuint) :: nil))))
+    (Sifthenelse (Etempvar _t'1 tint)
+      (Ssequence
+        (Sset _t'2
+          (Efield
+            (Ederef (Etempvar _bn (tptr (Tstruct _BorderNode noattr)))
+              (Tstruct _BorderNode noattr)) _suffixLink (tptr tvoid)))
+        (Sreturn (Some (Etempvar _t'2 (tptr tvoid)))))
+      (Sreturn (Some (Econst_int (Int.repr 0) tint))))))
+|}.
+
+Definition f_BN_ExportSuffixValue := {|
+  fn_return := (tptr tvoid);
+  fn_callconv := cc_default;
+  fn_params := ((_bn, (tptr (Tstruct _BorderNode noattr))) ::
+                (_key, (tptr (tptr (Tstruct _Key_T noattr)))) :: nil);
+  fn_vars := nil;
+  fn_temps := ((_ret_temp, (tptr tvoid)) ::
+               (_t'1, (tptr (Tstruct _Key_T noattr))) :: (_t'4, tuint) ::
+               (_t'3, (tptr tschar)) :: (_t'2, (tptr tschar)) :: nil);
+  fn_body :=
+(Ssequence
+  (Ssequence
+    (Sset _t'2
+      (Efield
+        (Ederef (Etempvar _bn (tptr (Tstruct _BorderNode noattr)))
+          (Tstruct _BorderNode noattr)) _keySuffix (tptr tschar)))
+    (Sifthenelse (Ebinop One (Etempvar _t'2 (tptr tschar))
+                   (Ecast (Econst_int (Int.repr 0) tint) (tptr tvoid)) tint)
+      (Ssequence
+        (Ssequence
+          (Ssequence
+            (Sset _t'3
+              (Efield
+                (Ederef (Etempvar _bn (tptr (Tstruct _BorderNode noattr)))
+                  (Tstruct _BorderNode noattr)) _keySuffix (tptr tschar)))
+            (Ssequence
+              (Sset _t'4
+                (Efield
+                  (Ederef (Etempvar _bn (tptr (Tstruct _BorderNode noattr)))
+                    (Tstruct _BorderNode noattr)) _keySuffixLength tuint))
+              (Scall (Some _t'1)
+                (Evar _move_key (Tfunction
+                                  (Tcons (tptr tschar) (Tcons tuint Tnil))
+                                  (tptr (Tstruct _Key_T noattr)) cc_default))
+                ((Etempvar _t'3 (tptr tschar)) :: (Etempvar _t'4 tuint) ::
+                 nil))))
+          (Sassign
+            (Ederef (Etempvar _key (tptr (tptr (Tstruct _Key_T noattr))))
+              (tptr (Tstruct _Key_T noattr)))
+            (Etempvar _t'1 (tptr (Tstruct _Key_T noattr)))))
+        (Ssequence
+          (Sassign
+            (Efield
+              (Ederef (Etempvar _bn (tptr (Tstruct _BorderNode noattr)))
+                (Tstruct _BorderNode noattr)) _keySuffix (tptr tschar))
+            (Econst_int (Int.repr 0) tint))
+          (Sassign
+            (Efield
+              (Ederef (Etempvar _bn (tptr (Tstruct _BorderNode noattr)))
+                (Tstruct _BorderNode noattr)) _keySuffixLength tuint)
+            (Econst_int (Int.repr 0) tint))))
+      (Sassign
+        (Ederef (Etempvar _key (tptr (tptr (Tstruct _Key_T noattr))))
+          (tptr (Tstruct _Key_T noattr))) (Econst_int (Int.repr 0) tint))))
+  (Ssequence
+    (Sset _ret_temp
+      (Efield
+        (Ederef (Etempvar _bn (tptr (Tstruct _BorderNode noattr)))
+          (Tstruct _BorderNode noattr)) _suffixLink (tptr tvoid)))
+    (Ssequence
+      (Sassign
+        (Efield
+          (Ederef (Etempvar _bn (tptr (Tstruct _BorderNode noattr)))
+            (Tstruct _BorderNode noattr)) _suffixLink (tptr tvoid))
+        (Econst_int (Int.repr 0) tint))
+      (Sreturn (Some (Etempvar _ret_temp (tptr tvoid)))))))
+|}.
+
+Definition f_BN_SetLink := {|
+  fn_return := tvoid;
+  fn_callconv := cc_default;
+  fn_params := ((_bn, (tptr (Tstruct _BorderNode noattr))) ::
+                (_val, (tptr tvoid)) :: nil);
+  fn_vars := nil;
+  fn_temps := ((_t'2, (tptr tschar)) :: (_t'1, (tptr tschar)) :: nil);
+  fn_body :=
+(Ssequence
+  (Ssequence
+    (Sset _t'1
+      (Efield
+        (Ederef (Etempvar _bn (tptr (Tstruct _BorderNode noattr)))
+          (Tstruct _BorderNode noattr)) _keySuffix (tptr tschar)))
+    (Sifthenelse (Ebinop One (Etempvar _t'1 (tptr tschar))
+                   (Ecast (Econst_int (Int.repr 0) tint) (tptr tvoid)) tint)
+      (Ssequence
+        (Sset _t'2
+          (Efield
+            (Ederef (Etempvar _bn (tptr (Tstruct _BorderNode noattr)))
+              (Tstruct _BorderNode noattr)) _keySuffix (tptr tschar)))
+        (Scall None
+          (Evar _free (Tfunction (Tcons (tptr tvoid) Tnil) tvoid cc_default))
+          ((Etempvar _t'2 (tptr tschar)) :: nil)))
+      Sskip))
+  (Ssequence
+    (Sassign
+      (Efield
+        (Ederef (Etempvar _bn (tptr (Tstruct _BorderNode noattr)))
+          (Tstruct _BorderNode noattr)) _keySuffix (tptr tschar))
+      (Econst_int (Int.repr 0) tint))
+    (Ssequence
+      (Sassign
+        (Efield
+          (Ederef (Etempvar _bn (tptr (Tstruct _BorderNode noattr)))
+            (Tstruct _BorderNode noattr)) _keySuffixLength tuint)
+        (Econst_int (Int.repr 0) tint))
+      (Sassign
+        (Efield
+          (Ederef (Etempvar _bn (tptr (Tstruct _BorderNode noattr)))
+            (Tstruct _BorderNode noattr)) _suffixLink (tptr tvoid))
+        (Etempvar _val (tptr tvoid))))))
+|}.
+
+Definition f_BN_GetLink := {|
+  fn_return := (tptr tvoid);
+  fn_callconv := cc_default;
+  fn_params := ((_bn, (tptr (Tstruct _BorderNode noattr))) :: nil);
+  fn_vars := nil;
+  fn_temps := ((_t'2, (tptr tschar)) :: (_t'1, (tptr tvoid)) :: nil);
+  fn_body :=
+(Ssequence
+  (Ssequence
+    (Sset _t'2
+      (Efield
+        (Ederef (Etempvar _bn (tptr (Tstruct _BorderNode noattr)))
+          (Tstruct _BorderNode noattr)) _keySuffix (tptr tschar)))
+    (Sifthenelse (Ebinop One (Etempvar _t'2 (tptr tschar))
+                   (Ecast (Econst_int (Int.repr 0) tint) (tptr tvoid)) tint)
+      (Sreturn (Some (Econst_int (Int.repr 0) tint)))
+      Sskip))
+  (Ssequence
+    (Sset _t'1
+      (Efield
+        (Ederef (Etempvar _bn (tptr (Tstruct _BorderNode noattr)))
+          (Tstruct _BorderNode noattr)) _suffixLink (tptr tvoid)))
+    (Sreturn (Some (Etempvar _t'1 (tptr tvoid))))))
+|}.
+
+Definition f_BN_HasSuffix := {|
+  fn_return := tint;
+  fn_callconv := cc_default;
+  fn_params := ((_bn, (tptr (Tstruct _BorderNode noattr))) :: nil);
+  fn_vars := nil;
+  fn_temps := ((_t'1, (tptr tschar)) :: nil);
+  fn_body :=
+(Ssequence
+  (Sset _t'1
+    (Efield
+      (Ederef (Etempvar _bn (tptr (Tstruct _BorderNode noattr)))
+        (Tstruct _BorderNode noattr)) _keySuffix (tptr tschar)))
+  (Sreturn (Some (Ebinop One (Etempvar _t'1 (tptr tschar))
+                   (Ecast (Econst_int (Int.repr 0) tint) (tptr tvoid)) tint))))
+|}.
+
+Definition f_BN_SetValue := {|
+  fn_return := tvoid;
+  fn_callconv := cc_default;
+  fn_params := ((_bn, (tptr (Tstruct _BorderNode noattr))) ::
+                (_key, (tptr (Tstruct _Key_T noattr))) ::
+                (_val, (tptr tvoid)) :: nil);
+  fn_vars := nil;
+  fn_temps := ((_t'4, tuint) :: (_t'3, (tptr tschar)) :: (_t'2, tuint) ::
+               (_t'1, tuint) :: nil);
+  fn_body :=
+(Ssequence
+  (Sset _t'1
+    (Efield
+      (Ederef (Etempvar _key (tptr (Tstruct _Key_T noattr)))
+        (Tstruct _Key_T noattr)) _len tuint))
+  (Sifthenelse (Ebinop Ogt (Etempvar _t'1 tuint)
+                 (Ecast (Esizeof tuint tuint) tint) tint)
+    (Ssequence
+      (Sset _t'3
+        (Efield
+          (Ederef (Etempvar _key (tptr (Tstruct _Key_T noattr)))
+            (Tstruct _Key_T noattr)) _content (tptr tschar)))
+      (Ssequence
+        (Sset _t'4
+          (Efield
+            (Ederef (Etempvar _key (tptr (Tstruct _Key_T noattr)))
+              (Tstruct _Key_T noattr)) _len tuint))
+        (Scall None
+          (Evar _BN_SetSuffixValue (Tfunction
+                                     (Tcons
+                                       (tptr (Tstruct _BorderNode noattr))
+                                       (Tcons (tptr tschar)
+                                         (Tcons tuint
+                                           (Tcons (tptr tvoid) Tnil)))) tvoid
+                                     cc_default))
+          ((Etempvar _bn (tptr (Tstruct _BorderNode noattr))) ::
+           (Ebinop Oadd (Etempvar _t'3 (tptr tschar))
+             (Ecast (Esizeof tuint tuint) tint) (tptr tschar)) ::
+           (Ebinop Osub (Etempvar _t'4 tuint)
+             (Ecast (Esizeof tuint tuint) tint) tuint) ::
+           (Etempvar _val (tptr tvoid)) :: nil))))
+    (Ssequence
+      (Sset _t'2
+        (Efield
+          (Ederef (Etempvar _key (tptr (Tstruct _Key_T noattr)))
+            (Tstruct _Key_T noattr)) _len tuint))
+      (Scall None
+        (Evar _BN_SetPrefixValue (Tfunction
+                                   (Tcons (tptr (Tstruct _BorderNode noattr))
+                                     (Tcons tint (Tcons (tptr tvoid) Tnil)))
+                                   tvoid cc_default))
+        ((Etempvar _bn (tptr (Tstruct _BorderNode noattr))) ::
+         (Etempvar _t'2 tuint) :: (Etempvar _val (tptr tvoid)) :: nil)))))
+|}.
+
+Definition f_Sempty := {|
+  fn_return := (tptr tvoid);
+  fn_callconv := cc_default;
+  fn_params := nil;
+  fn_vars := nil;
+  fn_temps := ((_new_index, (tptr tvoid)) :: (_t'1, (tptr tvoid)) :: nil);
+  fn_body :=
+(Ssequence
+  (Ssequence
+    (Scall (Some _t'1)
+      (Evar _surely_malloc (Tfunction (Tcons tuint Tnil) (tptr tvoid)
+                             cc_default))
+      ((Esizeof (tptr tvoid) tuint) :: nil))
+    (Sset _new_index (Etempvar _t'1 (tptr tvoid))))
+  (Sreturn (Some (Etempvar _new_index (tptr tvoid)))))
+|}.
+
+Definition f__make_cursor := {|
+  fn_return := tvoid;
+  fn_callconv := cc_default;
+  fn_params := ((_key, (tptr (Tstruct _Key_T noattr))) ::
+                (_index, (tptr tvoid)) ::
+                (_cursor, (tptr (Tstruct _Cursor_T noattr))) :: nil);
+  fn_vars := ((_slice, (Tstruct _CursorSlice_T noattr)) ::
+              (_slice__1, (Tstruct _CursorSlice_T noattr)) :: nil);
+  fn_temps := ((_keyslice, tuint) :: (_node_cursor, (tptr tvoid)) ::
+               (_obtained_keyslice, tuint) ::
+               (_bnode, (tptr (Tstruct _BorderNode noattr))) ::
+               (_subkey, (tptr (Tstruct _Key_T noattr))) ::
+               (_subindex, (tptr tvoid)) ::
+               (_subkey__1, (tptr (Tstruct _Key_T noattr))) ::
+               (_t'9, tint) :: (_t'8, (tptr (Tstruct _Key_T noattr))) ::
+               (_t'7, (tptr tvoid)) :: (_t'6, tint) ::
+               (_t'5, (tptr (Tstruct _Key_T noattr))) ::
+               (_t'4, (tptr tvoid)) :: (_t'3, tuint) ::
+               (_t'2, (tptr tvoid)) :: (_t'1, tuint) :: (_t'17, tuint) ::
+               (_t'16, (tptr tschar)) :: (_t'15, tuint) :: (_t'14, tuint) ::
+               (_t'13, (tptr tschar)) :: (_t'12, tuint) ::
+               (_t'11, (tptr tschar)) :: (_t'10, tuint) :: nil);
+  fn_body :=
+(Ssequence
+  (Ssequence
+    (Ssequence
+      (Sset _t'16
+        (Efield
+          (Ederef (Etempvar _key (tptr (Tstruct _Key_T noattr)))
+            (Tstruct _Key_T noattr)) _content (tptr tschar)))
+      (Ssequence
+        (Sset _t'17
+          (Efield
+            (Ederef (Etempvar _key (tptr (Tstruct _Key_T noattr)))
+              (Tstruct _Key_T noattr)) _len tuint))
+        (Scall (Some _t'1)
+          (Evar _UTIL_GetNextKeySlice (Tfunction
+                                        (Tcons (tptr tschar)
+                                          (Tcons tint Tnil)) tuint
+                                        cc_default))
+          ((Etempvar _t'16 (tptr tschar)) :: (Etempvar _t'17 tuint) :: nil))))
+    (Sset _keyslice (Etempvar _t'1 tuint)))
+  (Ssequence
+    (Ssequence
+      (Scall (Some _t'2)
+        (Evar _Imake_cursor (Tfunction
+                              (Tcons tuint (Tcons (tptr tvoid) Tnil))
+                              (tptr tvoid) cc_default))
+        ((Etempvar _keyslice tuint) :: (Etempvar _index (tptr tvoid)) :: nil))
+      (Sset _node_cursor (Etempvar _t'2 (tptr tvoid))))
+    (Ssequence
+      (Ssequence
+        (Scall (Some _t'3)
+          (Evar _Iget_key (Tfunction
+                            (Tcons (tptr tvoid) (Tcons (tptr tvoid) Tnil))
+                            tuint cc_default))
+          ((Etempvar _node_cursor (tptr tvoid)) ::
+           (Etempvar _index (tptr tvoid)) :: nil))
+        (Sset _obtained_keyslice (Etempvar _t'3 tuint)))
+      (Sifthenelse (Ebinop Oeq (Etempvar _keyslice tuint)
+                     (Etempvar _obtained_keyslice tuint) tint)
+        (Ssequence
+          (Sset _t'10
+            (Efield
+              (Ederef (Etempvar _key (tptr (Tstruct _Key_T noattr)))
+                (Tstruct _Key_T noattr)) _len tuint))
+          (Sifthenelse (Ebinop Ole (Etempvar _t'10 tuint)
+                         (Ecast (Esizeof tuint tuint) tint) tint)
+            (Ssequence
+              (Sset _t'15
+                (Efield
+                  (Ederef (Etempvar _key (tptr (Tstruct _Key_T noattr)))
+                    (Tstruct _Key_T noattr)) _len tuint))
+              (Scall None
+                (Evar _push_cursor (Tfunction
+                                     (Tcons (tptr tvoid)
+                                       (Tcons tuint
+                                         (Tcons
+                                           (tptr (Tstruct _Cursor_T noattr))
+                                           Tnil))) tvoid cc_default))
+                ((Etempvar _node_cursor (tptr tvoid)) ::
+                 (Etempvar _t'15 tuint) ::
+                 (Etempvar _cursor (tptr (Tstruct _Cursor_T noattr))) :: nil)))
+            (Ssequence
+              (Ssequence
+                (Scall (Some _t'4)
+                  (Evar _Iget_value (Tfunction
+                                      (Tcons (tptr tvoid)
+                                        (Tcons (tptr tvoid) Tnil))
+                                      (tptr tvoid) cc_default))
+                  ((Etempvar _node_cursor (tptr tvoid)) ::
+                   (Etempvar _index (tptr tvoid)) :: nil))
+                (Sset _bnode (Etempvar _t'4 (tptr tvoid))))
+              (Ssequence
+                (Scall (Some _t'9)
+                  (Evar _BN_HasSuffix (Tfunction
+                                        (Tcons
+                                          (tptr (Tstruct _BorderNode noattr))
+                                          Tnil) tint cc_default))
+                  ((Etempvar _bnode (tptr (Tstruct _BorderNode noattr))) ::
+                   nil))
+                (Sifthenelse (Etempvar _t'9 tint)
+                  (Ssequence
+                    (Sassign
+                      (Efield (Evar _slice (Tstruct _CursorSlice_T noattr))
+                        _node_cursor (tptr tvoid))
+                      (Etempvar _node_cursor (tptr tvoid)))
+                    (Ssequence
+                      (Ssequence
+                        (Ssequence
+                          (Sset _t'13
+                            (Efield
+                              (Ederef
+                                (Etempvar _key (tptr (Tstruct _Key_T noattr)))
+                                (Tstruct _Key_T noattr)) _content
+                              (tptr tschar)))
+                          (Ssequence
+                            (Sset _t'14
+                              (Efield
+                                (Ederef
+                                  (Etempvar _key (tptr (Tstruct _Key_T noattr)))
+                                  (Tstruct _Key_T noattr)) _len tuint))
+                            (Scall (Some _t'5)
+                              (Evar _new_key (Tfunction
+                                               (Tcons (tptr tschar)
+                                                 (Tcons tuint Tnil))
+                                               (tptr (Tstruct _Key_T noattr))
+                                               cc_default))
+                              ((Ebinop Oadd (Etempvar _t'13 (tptr tschar))
+                                 (Ecast (Esizeof tuint tuint) tint)
+                                 (tptr tschar)) ::
+                               (Ebinop Osub (Etempvar _t'14 tuint)
+                                 (Ecast (Esizeof tuint tuint) tint) tuint) ::
+                               nil))))
+                        (Sset _subkey
+                          (Etempvar _t'5 (tptr (Tstruct _Key_T noattr)))))
+                      (Ssequence
+                        (Scall (Some _t'6)
+                          (Evar _BN_CompareSuffix (Tfunction
+                                                    (Tcons
+                                                      (tptr (Tstruct _BorderNode noattr))
+                                                      (Tcons
+                                                        (tptr (Tstruct _Key_T noattr))
+                                                        Tnil)) tint
+                                                    cc_default))
+                          ((Etempvar _bnode (tptr (Tstruct _BorderNode noattr))) ::
+                           (Etempvar _subkey (tptr (Tstruct _Key_T noattr))) ::
+                           nil))
+                        (Sifthenelse (Etempvar _t'6 tint)
+                          (Scall None
+                            (Evar _push_cursor (Tfunction
+                                                 (Tcons (tptr tvoid)
+                                                   (Tcons tuint
+                                                     (Tcons
+                                                       (tptr (Tstruct _Cursor_T noattr))
+                                                       Tnil))) tvoid
+                                                 cc_default))
+                            ((Etempvar _node_cursor (tptr tvoid)) ::
+                             (Ebinop Oadd (Ecast (Esizeof tuint tuint) tint)
+                               (Econst_int (Int.repr 1) tint) tint) ::
+                             (Etempvar _cursor (tptr (Tstruct _Cursor_T noattr))) ::
+                             nil))
+                          (Scall None
+                            (Evar _push_cursor (Tfunction
+                                                 (Tcons (tptr tvoid)
+                                                   (Tcons tuint
+                                                     (Tcons
+                                                       (tptr (Tstruct _Cursor_T noattr))
+                                                       Tnil))) tvoid
+                                                 cc_default))
+                            ((Etempvar _node_cursor (tptr tvoid)) ::
+                             (Ebinop Oadd (Ecast (Esizeof tuint tuint) tint)
+                               (Econst_int (Int.repr 2) tint) tint) ::
+                             (Etempvar _cursor (tptr (Tstruct _Cursor_T noattr))) ::
+                             nil))))))
+                  (Ssequence
+                    (Ssequence
+                      (Scall (Some _t'7)
+                        (Evar _BN_GetLink (Tfunction
+                                            (Tcons
+                                              (tptr (Tstruct _BorderNode noattr))
+                                              Tnil) (tptr tvoid) cc_default))
+                        ((Etempvar _bnode (tptr (Tstruct _BorderNode noattr))) ::
+                         nil))
+                      (Sset _subindex (Etempvar _t'7 (tptr tvoid))))
+                    (Sifthenelse (Ebinop One
+                                   (Etempvar _subindex (tptr tvoid))
+                                   (Ecast (Econst_int (Int.repr 0) tint)
+                                     (tptr tvoid)) tint)
+                      (Ssequence
+                        (Sassign
+                          (Efield
+                            (Evar _slice__1 (Tstruct _CursorSlice_T noattr))
+                            _node_cursor (tptr tvoid))
+                          (Etempvar _node_cursor (tptr tvoid)))
+                        (Ssequence
+                          (Sassign
+                            (Efield
+                              (Evar _slice__1 (Tstruct _CursorSlice_T noattr))
+                              _bnode_cursor tuint)
+                            (Ebinop Oadd (Ecast (Esizeof tuint tuint) tint)
+                              (Econst_int (Int.repr 1) tint) tint))
+                          (Ssequence
+                            (Scall None
+                              (Evar _push_cursor (Tfunction
+                                                   (Tcons (tptr tvoid)
+                                                     (Tcons tuint
+                                                       (Tcons
+                                                         (tptr (Tstruct _Cursor_T noattr))
+                                                         Tnil))) tvoid
+                                                   cc_default))
+                              ((Etempvar _node_cursor (tptr tvoid)) ::
+                               (Ebinop Oadd
+                                 (Ecast (Esizeof tuint tuint) tint)
+                                 (Econst_int (Int.repr 1) tint) tint) ::
+                               (Etempvar _cursor (tptr (Tstruct _Cursor_T noattr))) ::
+                               nil))
+                            (Ssequence
+                              (Ssequence
+                                (Ssequence
+                                  (Sset _t'11
+                                    (Efield
+                                      (Ederef
+                                        (Etempvar _key (tptr (Tstruct _Key_T noattr)))
+                                        (Tstruct _Key_T noattr)) _content
+                                      (tptr tschar)))
+                                  (Ssequence
+                                    (Sset _t'12
+                                      (Efield
+                                        (Ederef
+                                          (Etempvar _key (tptr (Tstruct _Key_T noattr)))
+                                          (Tstruct _Key_T noattr)) _len
+                                        tuint))
+                                    (Scall (Some _t'8)
+                                      (Evar _new_key (Tfunction
+                                                       (Tcons (tptr tschar)
+                                                         (Tcons tuint Tnil))
+                                                       (tptr (Tstruct _Key_T noattr))
+                                                       cc_default))
+                                      ((Ebinop Oadd
+                                         (Etempvar _t'11 (tptr tschar))
+                                         (Ecast (Esizeof tuint tuint) tint)
+                                         (tptr tschar)) ::
+                                       (Ebinop Osub (Etempvar _t'12 tuint)
+                                         (Ecast (Esizeof tuint tuint) tint)
+                                         tuint) :: nil))))
+                                (Sset _subkey__1
+                                  (Etempvar _t'8 (tptr (Tstruct _Key_T noattr)))))
+                              (Scall None
+                                (Evar __make_cursor (Tfunction
+                                                      (Tcons
+                                                        (tptr (Tstruct _Key_T noattr))
+                                                        (Tcons (tptr tvoid)
+                                                          (Tcons
+                                                            (tptr (Tstruct _Cursor_T noattr))
+                                                            Tnil))) tvoid
+                                                      cc_default))
+                                ((Etempvar _subkey__1 (tptr (Tstruct _Key_T noattr))) ::
+                                 (Etempvar _subindex (tptr tvoid)) ::
+                                 (Etempvar _cursor (tptr (Tstruct _Cursor_T noattr))) ::
+                                 nil))))))
+                      Sskip)))))))
+        Sskip))))
+|}.
+
+Definition f_Smake_cursor := {|
+  fn_return := (tptr (Tstruct _Cursor_T noattr));
+  fn_callconv := cc_default;
+  fn_params := ((_key, (tptr (Tstruct _Key_T noattr))) ::
+                (_index, (tptr tvoid)) :: nil);
+  fn_vars := nil;
+  fn_temps := ((_cursor, (tptr (Tstruct _Cursor_T noattr))) ::
+               (_t'2, (tptr (Tstruct _Cursor_T noattr))) ::
+               (_t'1, (tptr (Tstruct _Cursor_T noattr))) :: nil);
+  fn_body :=
+(Ssequence
+  (Ssequence
+    (Scall (Some _t'1)
+      (Evar _new_cursor (Tfunction Tnil (tptr (Tstruct _Cursor_T noattr))
+                          cc_default)) nil)
+    (Sset _cursor (Etempvar _t'1 (tptr (Tstruct _Cursor_T noattr)))))
+  (Ssequence
+    (Ssequence
+      (Scall (Some _t'2)
+        (Evar _new_cursor (Tfunction Tnil (tptr (Tstruct _Cursor_T noattr))
+                            cc_default)) nil)
+      (Scall None
+        (Evar __make_cursor (Tfunction
+                              (Tcons (tptr (Tstruct _Key_T noattr))
+                                (Tcons (tptr tvoid)
+                                  (Tcons (tptr (Tstruct _Cursor_T noattr))
+                                    Tnil))) tvoid cc_default))
+        ((Etempvar _key (tptr (Tstruct _Key_T noattr))) ::
+         (Etempvar _index (tptr tvoid)) ::
+         (Etempvar _t'2 (tptr (Tstruct _Cursor_T noattr))) :: nil)))
+    (Sreturn (Some (Etempvar _cursor (tptr (Tstruct _Cursor_T noattr)))))))
+|}.
+
+Definition composites : list composite_definition :=
+(Composite _Key_T Struct
+   ((_content, (tptr tschar)) :: (_len, tuint) :: nil)
+   noattr ::
+ Composite _CursorSlice_T Struct
+   ((_node_cursor, (tptr tvoid)) :: (_bnode_cursor, tuint) :: nil)
+   noattr ::
+ Composite _Cursor_T Struct
+   ((_capacity, tuint) :: (_size, tuint) ::
+    (_content, (tptr (Tstruct _CursorSlice_T noattr))) :: nil)
+   noattr ::
+ Composite _BorderNode Struct
+   ((_prefixLinks, (tarray (tptr tvoid) 4)) :: (_suffixLink, (tptr tvoid)) ::
+    (_keySuffix, (tptr tschar)) :: (_keySuffixLength, tuint) :: nil)
+   noattr :: nil).
+
+Definition global_definitions : list (ident * globdef fundef type) :=
+((___builtin_ais_annot,
+   Gfun(External (EF_builtin "__builtin_ais_annot"
+                   (mksignature (AST.Tint :: nil) None
+                     {|cc_vararg:=true; cc_unproto:=false; cc_structret:=false|}))
+     (Tcons (tptr tschar) Tnil) tvoid
+     {|cc_vararg:=true; cc_unproto:=false; cc_structret:=false|})) ::
+ (___builtin_bswap,
+   Gfun(External (EF_builtin "__builtin_bswap"
+                   (mksignature (AST.Tint :: nil) (Some AST.Tint) cc_default))
+     (Tcons tuint Tnil) tuint cc_default)) ::
+ (___builtin_bswap32,
+   Gfun(External (EF_builtin "__builtin_bswap32"
+                   (mksignature (AST.Tint :: nil) (Some AST.Tint) cc_default))
+     (Tcons tuint Tnil) tuint cc_default)) ::
+ (___builtin_bswap16,
+   Gfun(External (EF_builtin "__builtin_bswap16"
+                   (mksignature (AST.Tint :: nil) (Some AST.Tint) cc_default))
+     (Tcons tushort Tnil) tushort cc_default)) ::
+ (___builtin_fabs,
+   Gfun(External (EF_builtin "__builtin_fabs"
+                   (mksignature (AST.Tfloat :: nil) (Some AST.Tfloat)
+                     cc_default)) (Tcons tdouble Tnil) tdouble cc_default)) ::
+ (___builtin_fsqrt,
+   Gfun(External (EF_builtin "__builtin_fsqrt"
+                   (mksignature (AST.Tfloat :: nil) (Some AST.Tfloat)
+                     cc_default)) (Tcons tdouble Tnil) tdouble cc_default)) ::
+ (___builtin_memcpy_aligned,
+   Gfun(External (EF_builtin "__builtin_memcpy_aligned"
+                   (mksignature
+                     (AST.Tint :: AST.Tint :: AST.Tint :: AST.Tint :: nil)
+                     None cc_default))
+     (Tcons (tptr tvoid)
+       (Tcons (tptr tvoid) (Tcons tuint (Tcons tuint Tnil)))) tvoid
+     cc_default)) ::
+ (___builtin_annot,
+   Gfun(External (EF_builtin "__builtin_annot"
+                   (mksignature (AST.Tint :: nil) None
+                     {|cc_vararg:=true; cc_unproto:=false; cc_structret:=false|}))
+     (Tcons (tptr tschar) Tnil) tvoid
+     {|cc_vararg:=true; cc_unproto:=false; cc_structret:=false|})) ::
+ (___builtin_annot_intval,
+   Gfun(External (EF_builtin "__builtin_annot_intval"
+                   (mksignature (AST.Tint :: AST.Tint :: nil) (Some AST.Tint)
+                     cc_default)) (Tcons (tptr tschar) (Tcons tint Tnil))
+     tint cc_default)) ::
+ (___builtin_membar,
+   Gfun(External (EF_builtin "__builtin_membar"
+                   (mksignature nil None cc_default)) Tnil tvoid cc_default)) ::
+ (___builtin_va_start,
+   Gfun(External (EF_builtin "__builtin_va_start"
+                   (mksignature (AST.Tint :: nil) None cc_default))
+     (Tcons (tptr tvoid) Tnil) tvoid cc_default)) ::
+ (___builtin_va_arg,
+   Gfun(External (EF_builtin "__builtin_va_arg"
+                   (mksignature (AST.Tint :: AST.Tint :: nil) None
+                     cc_default)) (Tcons (tptr tvoid) (Tcons tuint Tnil))
+     tvoid cc_default)) ::
+ (___builtin_va_copy,
+   Gfun(External (EF_builtin "__builtin_va_copy"
+                   (mksignature (AST.Tint :: AST.Tint :: nil) None
+                     cc_default))
+     (Tcons (tptr tvoid) (Tcons (tptr tvoid) Tnil)) tvoid cc_default)) ::
+ (___builtin_va_end,
+   Gfun(External (EF_builtin "__builtin_va_end"
+                   (mksignature (AST.Tint :: nil) None cc_default))
+     (Tcons (tptr tvoid) Tnil) tvoid cc_default)) ::
+ (___compcert_va_int32,
+   Gfun(External (EF_external "__compcert_va_int32"
+                   (mksignature (AST.Tint :: nil) (Some AST.Tint) cc_default))
+     (Tcons (tptr tvoid) Tnil) tuint cc_default)) ::
+ (___compcert_va_int64,
+   Gfun(External (EF_external "__compcert_va_int64"
+                   (mksignature (AST.Tint :: nil) (Some AST.Tlong)
+                     cc_default)) (Tcons (tptr tvoid) Tnil) tulong
+     cc_default)) ::
+ (___compcert_va_float64,
+   Gfun(External (EF_external "__compcert_va_float64"
+                   (mksignature (AST.Tint :: nil) (Some AST.Tfloat)
+                     cc_default)) (Tcons (tptr tvoid) Tnil) tdouble
+     cc_default)) ::
+ (___compcert_va_composite,
+   Gfun(External (EF_external "__compcert_va_composite"
+                   (mksignature (AST.Tint :: AST.Tint :: nil) (Some AST.Tint)
+                     cc_default)) (Tcons (tptr tvoid) (Tcons tuint Tnil))
+     (tptr tvoid) cc_default)) ::
+ (___compcert_i64_dtos,
+   Gfun(External (EF_runtime "__compcert_i64_dtos"
+                   (mksignature (AST.Tfloat :: nil) (Some AST.Tlong)
+                     cc_default)) (Tcons tdouble Tnil) tlong cc_default)) ::
+ (___compcert_i64_dtou,
+   Gfun(External (EF_runtime "__compcert_i64_dtou"
+                   (mksignature (AST.Tfloat :: nil) (Some AST.Tlong)
+                     cc_default)) (Tcons tdouble Tnil) tulong cc_default)) ::
+ (___compcert_i64_stod,
+   Gfun(External (EF_runtime "__compcert_i64_stod"
+                   (mksignature (AST.Tlong :: nil) (Some AST.Tfloat)
+                     cc_default)) (Tcons tlong Tnil) tdouble cc_default)) ::
+ (___compcert_i64_utod,
+   Gfun(External (EF_runtime "__compcert_i64_utod"
+                   (mksignature (AST.Tlong :: nil) (Some AST.Tfloat)
+                     cc_default)) (Tcons tulong Tnil) tdouble cc_default)) ::
+ (___compcert_i64_stof,
+   Gfun(External (EF_runtime "__compcert_i64_stof"
+                   (mksignature (AST.Tlong :: nil) (Some AST.Tsingle)
+                     cc_default)) (Tcons tlong Tnil) tfloat cc_default)) ::
+ (___compcert_i64_utof,
+   Gfun(External (EF_runtime "__compcert_i64_utof"
+                   (mksignature (AST.Tlong :: nil) (Some AST.Tsingle)
+                     cc_default)) (Tcons tulong Tnil) tfloat cc_default)) ::
+ (___compcert_i64_sdiv,
+   Gfun(External (EF_runtime "__compcert_i64_sdiv"
+                   (mksignature (AST.Tlong :: AST.Tlong :: nil)
+                     (Some AST.Tlong) cc_default))
+     (Tcons tlong (Tcons tlong Tnil)) tlong cc_default)) ::
+ (___compcert_i64_udiv,
+   Gfun(External (EF_runtime "__compcert_i64_udiv"
+                   (mksignature (AST.Tlong :: AST.Tlong :: nil)
+                     (Some AST.Tlong) cc_default))
+     (Tcons tulong (Tcons tulong Tnil)) tulong cc_default)) ::
+ (___compcert_i64_smod,
+   Gfun(External (EF_runtime "__compcert_i64_smod"
+                   (mksignature (AST.Tlong :: AST.Tlong :: nil)
+                     (Some AST.Tlong) cc_default))
+     (Tcons tlong (Tcons tlong Tnil)) tlong cc_default)) ::
+ (___compcert_i64_umod,
+   Gfun(External (EF_runtime "__compcert_i64_umod"
+                   (mksignature (AST.Tlong :: AST.Tlong :: nil)
+                     (Some AST.Tlong) cc_default))
+     (Tcons tulong (Tcons tulong Tnil)) tulong cc_default)) ::
+ (___compcert_i64_shl,
+   Gfun(External (EF_runtime "__compcert_i64_shl"
+                   (mksignature (AST.Tlong :: AST.Tint :: nil)
+                     (Some AST.Tlong) cc_default))
+     (Tcons tlong (Tcons tint Tnil)) tlong cc_default)) ::
+ (___compcert_i64_shr,
+   Gfun(External (EF_runtime "__compcert_i64_shr"
+                   (mksignature (AST.Tlong :: AST.Tint :: nil)
+                     (Some AST.Tlong) cc_default))
+     (Tcons tulong (Tcons tint Tnil)) tulong cc_default)) ::
+ (___compcert_i64_sar,
+   Gfun(External (EF_runtime "__compcert_i64_sar"
+                   (mksignature (AST.Tlong :: AST.Tint :: nil)
+                     (Some AST.Tlong) cc_default))
+     (Tcons tlong (Tcons tint Tnil)) tlong cc_default)) ::
+ (___compcert_i64_smulh,
+   Gfun(External (EF_runtime "__compcert_i64_smulh"
+                   (mksignature (AST.Tlong :: AST.Tlong :: nil)
+                     (Some AST.Tlong) cc_default))
+     (Tcons tlong (Tcons tlong Tnil)) tlong cc_default)) ::
+ (___compcert_i64_umulh,
+   Gfun(External (EF_runtime "__compcert_i64_umulh"
+                   (mksignature (AST.Tlong :: AST.Tlong :: nil)
+                     (Some AST.Tlong) cc_default))
+     (Tcons tulong (Tcons tulong Tnil)) tulong cc_default)) ::
+ (___builtin_bswap64,
+   Gfun(External (EF_builtin "__builtin_bswap64"
+                   (mksignature (AST.Tlong :: nil) (Some AST.Tlong)
+                     cc_default)) (Tcons tulong Tnil) tulong cc_default)) ::
+ (___builtin_clz,
+   Gfun(External (EF_builtin "__builtin_clz"
+                   (mksignature (AST.Tint :: nil) (Some AST.Tint) cc_default))
+     (Tcons tuint Tnil) tint cc_default)) ::
+ (___builtin_clzl,
+   Gfun(External (EF_builtin "__builtin_clzl"
+                   (mksignature (AST.Tint :: nil) (Some AST.Tint) cc_default))
+     (Tcons tuint Tnil) tint cc_default)) ::
+ (___builtin_clzll,
+   Gfun(External (EF_builtin "__builtin_clzll"
+                   (mksignature (AST.Tlong :: nil) (Some AST.Tint)
+                     cc_default)) (Tcons tulong Tnil) tint cc_default)) ::
+ (___builtin_ctz,
+   Gfun(External (EF_builtin "__builtin_ctz"
+                   (mksignature (AST.Tint :: nil) (Some AST.Tint) cc_default))
+     (Tcons tuint Tnil) tint cc_default)) ::
+ (___builtin_ctzl,
+   Gfun(External (EF_builtin "__builtin_ctzl"
+                   (mksignature (AST.Tint :: nil) (Some AST.Tint) cc_default))
+     (Tcons tuint Tnil) tint cc_default)) ::
+ (___builtin_ctzll,
+   Gfun(External (EF_builtin "__builtin_ctzll"
+                   (mksignature (AST.Tlong :: nil) (Some AST.Tint)
+                     cc_default)) (Tcons tulong Tnil) tint cc_default)) ::
+ (___builtin_fmax,
+   Gfun(External (EF_builtin "__builtin_fmax"
+                   (mksignature (AST.Tfloat :: AST.Tfloat :: nil)
+                     (Some AST.Tfloat) cc_default))
+     (Tcons tdouble (Tcons tdouble Tnil)) tdouble cc_default)) ::
+ (___builtin_fmin,
+   Gfun(External (EF_builtin "__builtin_fmin"
+                   (mksignature (AST.Tfloat :: AST.Tfloat :: nil)
+                     (Some AST.Tfloat) cc_default))
+     (Tcons tdouble (Tcons tdouble Tnil)) tdouble cc_default)) ::
+ (___builtin_fmadd,
+   Gfun(External (EF_builtin "__builtin_fmadd"
+                   (mksignature
+                     (AST.Tfloat :: AST.Tfloat :: AST.Tfloat :: nil)
+                     (Some AST.Tfloat) cc_default))
+     (Tcons tdouble (Tcons tdouble (Tcons tdouble Tnil))) tdouble
+     cc_default)) ::
+ (___builtin_fmsub,
+   Gfun(External (EF_builtin "__builtin_fmsub"
+                   (mksignature
+                     (AST.Tfloat :: AST.Tfloat :: AST.Tfloat :: nil)
+                     (Some AST.Tfloat) cc_default))
+     (Tcons tdouble (Tcons tdouble (Tcons tdouble Tnil))) tdouble
+     cc_default)) ::
+ (___builtin_fnmadd,
+   Gfun(External (EF_builtin "__builtin_fnmadd"
+                   (mksignature
+                     (AST.Tfloat :: AST.Tfloat :: AST.Tfloat :: nil)
+                     (Some AST.Tfloat) cc_default))
+     (Tcons tdouble (Tcons tdouble (Tcons tdouble Tnil))) tdouble
+     cc_default)) ::
+ (___builtin_fnmsub,
+   Gfun(External (EF_builtin "__builtin_fnmsub"
+                   (mksignature
+                     (AST.Tfloat :: AST.Tfloat :: AST.Tfloat :: nil)
+                     (Some AST.Tfloat) cc_default))
+     (Tcons tdouble (Tcons tdouble (Tcons tdouble Tnil))) tdouble
+     cc_default)) ::
+ (___builtin_read16_reversed,
+   Gfun(External (EF_builtin "__builtin_read16_reversed"
+                   (mksignature (AST.Tint :: nil) (Some AST.Tint) cc_default))
+     (Tcons (tptr tushort) Tnil) tushort cc_default)) ::
+ (___builtin_read32_reversed,
+   Gfun(External (EF_builtin "__builtin_read32_reversed"
+                   (mksignature (AST.Tint :: nil) (Some AST.Tint) cc_default))
+     (Tcons (tptr tuint) Tnil) tuint cc_default)) ::
+ (___builtin_write16_reversed,
+   Gfun(External (EF_builtin "__builtin_write16_reversed"
+                   (mksignature (AST.Tint :: AST.Tint :: nil) None
+                     cc_default)) (Tcons (tptr tushort) (Tcons tushort Tnil))
+     tvoid cc_default)) ::
+ (___builtin_write32_reversed,
+   Gfun(External (EF_builtin "__builtin_write32_reversed"
+                   (mksignature (AST.Tint :: AST.Tint :: nil) None
+                     cc_default)) (Tcons (tptr tuint) (Tcons tuint Tnil))
+     tvoid cc_default)) ::
+ (___builtin_nop,
+   Gfun(External (EF_builtin "__builtin_nop"
+                   (mksignature nil None cc_default)) Tnil tvoid cc_default)) ::
+ (___builtin_debug,
+   Gfun(External (EF_external "__builtin_debug"
+                   (mksignature (AST.Tint :: nil) None
+                     {|cc_vararg:=true; cc_unproto:=false; cc_structret:=false|}))
+     (Tcons tint Tnil) tvoid
+     {|cc_vararg:=true; cc_unproto:=false; cc_structret:=false|})) ::
+ (_malloc,
+   Gfun(External EF_malloc (Tcons tuint Tnil) (tptr tvoid) cc_default)) ::
+ (_free, Gfun(External EF_free (Tcons (tptr tvoid) Tnil) tvoid cc_default)) ::
+ (_exit,
+   Gfun(External (EF_external "exit"
+                   (mksignature (AST.Tint :: nil) None cc_default))
+     (Tcons tint Tnil) tvoid cc_default)) ::
+ (_Imake_cursor,
+   Gfun(External (EF_external "Imake_cursor"
+                   (mksignature (AST.Tint :: AST.Tint :: nil) (Some AST.Tint)
+                     cc_default)) (Tcons tuint (Tcons (tptr tvoid) Tnil))
+     (tptr tvoid) cc_default)) ::
+ (_Iget_key,
+   Gfun(External (EF_external "Iget_key"
+                   (mksignature (AST.Tint :: AST.Tint :: nil) (Some AST.Tint)
+                     cc_default))
+     (Tcons (tptr tvoid) (Tcons (tptr tvoid) Tnil)) tuint cc_default)) ::
+ (_Iget_value,
+   Gfun(External (EF_external "Iget_value"
+                   (mksignature (AST.Tint :: AST.Tint :: nil) (Some AST.Tint)
+                     cc_default))
+     (Tcons (tptr tvoid) (Tcons (tptr tvoid) Tnil)) (tptr tvoid) cc_default)) ::
+ (_surely_malloc, Gfun(Internal f_surely_malloc)) ::
+ (_push_cursor, Gfun(Internal f_push_cursor)) ::
+ (_pop_cursor, Gfun(Internal f_pop_cursor)) ::
+ (_new_cursor, Gfun(Internal f_new_cursor)) ::
+ (_UTIL_GetNextKeySlice, Gfun(Internal f_UTIL_GetNextKeySlice)) ::
+ (_UTIL_StrEqual, Gfun(Internal f_UTIL_StrEqual)) ::
+ (_new_key, Gfun(Internal f_new_key)) ::
+ (_move_key, Gfun(Internal f_move_key)) ::
+ (_BN_NewBorderNode, Gfun(Internal f_BN_NewBorderNode)) ::
+ (_BN_FreeBorderNode, Gfun(Internal f_BN_FreeBorderNode)) ::
+ (_BN_SetPrefixValue, Gfun(Internal f_BN_SetPrefixValue)) ::
+ (_BN_GetPrefixValue, Gfun(Internal f_BN_GetPrefixValue)) ::
+ (_BN_SetSuffixValue, Gfun(Internal f_BN_SetSuffixValue)) ::
+ (_BN_TestSuffix, Gfun(Internal f_BN_TestSuffix)) ::
+ (_BN_GetSuffixValue, Gfun(Internal f_BN_GetSuffixValue)) ::
+ (_BN_ExportSuffixValue, Gfun(Internal f_BN_ExportSuffixValue)) ::
+ (_BN_SetLink, Gfun(Internal f_BN_SetLink)) ::
+ (_BN_GetLink, Gfun(Internal f_BN_GetLink)) ::
+ (_BN_HasSuffix, Gfun(Internal f_BN_HasSuffix)) ::
+ (_BN_SetValue, Gfun(Internal f_BN_SetValue)) ::
+ (_BN_CompareSuffix,
+   Gfun(External (EF_external "BN_CompareSuffix"
+                   (mksignature (AST.Tint :: AST.Tint :: nil) (Some AST.Tint)
+                     cc_default))
+     (Tcons (tptr (Tstruct _BorderNode noattr))
+       (Tcons (tptr (Tstruct _Key_T noattr)) Tnil)) tint cc_default)) ::
+ (_Sempty, Gfun(Internal f_Sempty)) ::
+ (__make_cursor, Gfun(Internal f__make_cursor)) ::
+ (_Smake_cursor, Gfun(Internal f_Smake_cursor)) :: nil).
+
+Definition public_idents : list ident :=
+(_Smake_cursor :: __make_cursor :: _Sempty :: _BN_CompareSuffix ::
+ _BN_SetValue :: _BN_HasSuffix :: _BN_GetLink :: _BN_SetLink ::
+ _BN_ExportSuffixValue :: _BN_GetSuffixValue :: _BN_TestSuffix ::
+ _BN_SetSuffixValue :: _BN_GetPrefixValue :: _BN_SetPrefixValue ::
+ _BN_FreeBorderNode :: _BN_NewBorderNode :: _move_key :: _new_key ::
+ _UTIL_StrEqual :: _UTIL_GetNextKeySlice :: _new_cursor :: _pop_cursor ::
+ _push_cursor :: _surely_malloc :: _Iget_value :: _Iget_key ::
+ _Imake_cursor :: _exit :: _free :: _malloc :: ___builtin_debug ::
+ ___builtin_nop :: ___builtin_write32_reversed ::
+ ___builtin_write16_reversed :: ___builtin_read32_reversed ::
+ ___builtin_read16_reversed :: ___builtin_fnmsub :: ___builtin_fnmadd ::
+ ___builtin_fmsub :: ___builtin_fmadd :: ___builtin_fmin ::
+ ___builtin_fmax :: ___builtin_ctzll :: ___builtin_ctzl :: ___builtin_ctz ::
+ ___builtin_clzll :: ___builtin_clzl :: ___builtin_clz ::
+ ___builtin_bswap64 :: ___compcert_i64_umulh :: ___compcert_i64_smulh ::
+ ___compcert_i64_sar :: ___compcert_i64_shr :: ___compcert_i64_shl ::
+ ___compcert_i64_umod :: ___compcert_i64_smod :: ___compcert_i64_udiv ::
+ ___compcert_i64_sdiv :: ___compcert_i64_utof :: ___compcert_i64_stof ::
+ ___compcert_i64_utod :: ___compcert_i64_stod :: ___compcert_i64_dtou ::
+ ___compcert_i64_dtos :: ___compcert_va_composite ::
+ ___compcert_va_float64 :: ___compcert_va_int64 :: ___compcert_va_int32 ::
+ ___builtin_va_end :: ___builtin_va_copy :: ___builtin_va_arg ::
+ ___builtin_va_start :: ___builtin_membar :: ___builtin_annot_intval ::
+ ___builtin_annot :: ___builtin_memcpy_aligned :: ___builtin_fsqrt ::
+ ___builtin_fabs :: ___builtin_bswap16 :: ___builtin_bswap32 ::
+ ___builtin_bswap :: ___builtin_ais_annot :: nil).
+
+Definition prog : Clight.program := 
+  mkprogram composites global_definitions public_idents _main Logic.I.
+
+
