verif/trie/prog.v
@@ -1,5 +1,5 @@
 Require Export VST.floyd.proofauto.
-Require Export DB.clight.verifiable.
+Require Export DB.clight.index_string.
 
 Instance CompSpecs : compspecs. make_compspecs prog. Defined.
 Definition Vprog : varspecs. mk_varspecs prog. Defined.
