verif/trie/verif/verif_surely_malloc.v
@@ -2,7 +2,6 @@
 
 Require Import VST.floyd.proofauto.
 Require Import VST.floyd.library.
-Require Import DB.clight.verifiable.
 Require Import DB.specs.
 
 Definition Gprog : funspecs :=
